-

coq/Puiseux_series.v
@@ -1,4 +1,4 @@
-(* $Id: Puiseux_series.v,v 1.89 2013-08-02 02:20:43 deraugla Exp $ *)
+(* $Id: Puiseux_series.v,v 1.90 2013-08-02 06:39:17 deraugla Exp $ *)
 
 Require Import Utf8.
 Require Import QArith.
@@ -47,20 +47,15 @@ Definition normal l cd ps :=
      ps_comden := l |}.
 
 Inductive eq_ps : puiseux_series α → puiseux_series α → Prop :=
-  | eq_ps_stretched_l : ∀ k ps₁ ps₂,
+  | eq_ps_base : ∀ k ps₁ ps₂,
       eq_series fld
         (stretch_series (Pos.to_nat k) (ps_terms ps₁))
         (ps_terms ps₂)
       → ps_valnum ps₁ = ps_valnum ps₂
         → ps_comden ps₁ = (k * ps_comden ps₂)%positive
            → eq_ps ps₁ ps₂
-  | eq_ps_stretched_r : ∀ k ps₁ ps₂,
-      eq_series fld
-        (ps_terms ps₁)
-        (stretch_series (Pos.to_nat k) (ps_terms ps₂))
-      → ps_valnum ps₁ = ps_valnum ps₂
-        → (k * ps_comden ps₁)%positive = ps_comden ps₂
-           → eq_ps ps₁ ps₂.
+  | eq_ps_symm : ∀ ps₁ ps₂,
+      eq_ps ps₁ ps₂ → eq_ps ps₂ ps₁.
 
 Notation "a ≈ b" := (eq_ps a b) (at level 70).
 Notation "a ≃ b" := (eq_series fld a b) (at level 70).
@@ -84,10 +79,8 @@ Qed.
 Theorem eq_ps_sym : symmetric _ eq_ps.
 Proof.
 intros ps₁ ps₂ H.
-inversion H; subst.
- eapply eq_ps_stretched_r; symmetry; eassumption.
-
- eapply eq_ps_stretched_l; symmetry; eassumption.
+inversion H; subst; [ idtac | eassumption ].
+eapply eq_ps_symm, eq_ps_base; eassumption.
 Qed.
 
 Lemma stretch_stretch_series : ∀ a b s,
@@ -155,9 +148,7 @@ Proof.
 intros ps₁ ps₂ ps₃ H₁ H₂.
 inversion H₁ as [k₁| k₁]; subst.
  inversion H₂ as [k₂| k₂]; subst.
-  apply eq_ps_sym.
-  apply eq_ps_stretched_r with (k := (k₁ * k₂)%positive).
-   symmetry.
+  apply eq_ps_base with (k := (k₁ * k₂)%positive).
    etransitivity; [ idtac | eassumption ].
    rewrite Pos2Nat.inj_mul.
    rewrite mult_comm.
@@ -168,10 +159,8 @@ inversion H₁ as [k₁| k₁]; subst.
 
     apply pos_to_nat_ne_0.
 
-   symmetry.
    etransitivity; eassumption.
 
-   symmetry.
    rewrite <- Pos.mul_assoc, <- H4; assumption.
 bbb.
 
